$$
\tilde{A^T} = 
\begin{pmatrix}
a_{11}=(-1)^{1+1} 
* \begin{vmatrix} a_{22} & a_{32} \\ a_{23} & a_{33} \end{vmatrix} 
& 
a_{12}=(-1)^{1+2} 
* \begin{vmatrix} a_{12} & a_{32} \\ a_{13} & a_{33} \end{vmatrix} 
&
a_{13}=(-1)^{1+3} 
* \begin{vmatrix} a_{21} & a_{22} \\ a_{31} & a_{32} \end{vmatrix} 
\\ \\ 
a_{21}=(-1)^{1+2} 
* \begin{vmatrix} a_{12} & a_{13} \\ a_{32} & a_{33} \end{vmatrix} 
& 
a_{22}=(-1)^{2+2} 
* \begin{vmatrix} a_{11} & a_{13} \\ a_{31} & a_{33} \end{vmatrix} 
& 
a_{23}=(-1)^{2+3} 
* \begin{vmatrix} a_{11} & a_{12} \\ a_{31} & a_{32} \end{vmatrix} 
\\ \\ 
a_{31}=(-1)^{3+1} 
* \begin{vmatrix} a_{12} & a_{13} \\ a_{22} & a_{23} \end{vmatrix} 
& 
a_{32}=(-1)^{3+2} 
* \begin{vmatrix} a_{11} & a_{13} \\ a_{21} & a_{23} \end{vmatrix} 
& 
a_{33}=(-1)^{3+3} 
* \begin{vmatrix} a_{11} & a_{12} \\ a_{21} & a_{22} \end{vmatrix}
\end{pmatrix}
$$